theories/case_studies/tossCoin.v
@@ -17,18 +17,21 @@ From affect.logic Require Import tactics.
 
 (* Make all the definitions opaque so that we do not rely on their definition in the model to show that the programs are well-typed terms. *)
 Opaque sem_typed sem_typed_val ty_le row_le sig_le row_type_sub row_env_sub.
-Opaque sem_ty_bot sem_ty_unit sem_ty_bool sem_ty_int sem_ty_string sem_ty_top sem_ty_mbang env_mbang sem_ty_ref_cpy sem_ty_ref sem_ty_prod sem_ty_sum sem_ty_arr sem_ty_type_forall sem_ty_row_forall sem_ty_exists sem_ty_rec sem_ty_option sem_ty_list.
+Opaque sem_ty_bot sem_ty_unit sem_ty_bool sem_ty_int sem_ty_top sem_ty_mbang env_mbang sem_ty_ref_cpy sem_ty_ref sem_ty_prod sem_ty_sum sem_ty_arr sem_ty_type_forall sem_ty_row_forall sem_ty_exists sem_ty_rec sem_ty_option sem_ty_list.
 Opaque sem_sig_eff sem_sig_flip_mbang.
 Opaque sem_row_nil sem_row_flip_mbang sem_row_cons sem_row_rec.
 
-(* The tossCoin example from paper Soundly Hanlding Linearity by Tang et al. *)
+(* The tossCoin example from paper Soundly Handling Linearity by Tang et al. *)
+(* Note that we don't support strings natively but we encode them on the meta-level as integers *)  
 Definition tossCoin : val := 
   (λ: "g", let: "b" := "g" #() in 
-           if: "b" then #(LitStr "heads") else #(LitStr "tails"))%V.
+           if: "b" then #(Pos.to_nat (encode "heads")) else #(Pos.to_nat (encode "tails")))%V.
 
 Section typing.
 
   Context `{!heapGS Σ}.
+
+  Definition Str : sem_ty Σ := sem_ty_int.
 
   Definition tossCoin_ty : sem_ty Σ := 
     (∀ᵣ θ, (𝟙 -{ θ }-> 𝔹) -{ θ }-> Str)%T.
@@ -44,7 +47,7 @@ Section typing.
         iApply sem_typed_var'. }
       iApply sem_typed_unit'.
     - iApply sem_typed_if; first iApply sem_typed_var';
-      iApply sem_typed_string'.
+      iApply sem_typed_int'.
   Qed.
 
 End typing.
