README.md
@@ -20,16 +20,16 @@ eval "$(opam env --switch=affect)"
 ```
 
 `Affect` relies on `coq-hazel` a separation logic library for effect handlers. 
-To install `coq-hazel` we need to manually fetch it and apply the patch `hazel.patch` (this can take 5-10 minutes).
-Ignore the Licence warning.
+To install `coq-hazel` we need to manually fetch it and apply three patches (this can take 5-10 minutes).
 ```bash
 git clone https://gitlab.inria.fr/cambium/hazel
 ## If gitlab.inria.fr is down use local hazel copy: 
 # tar xzf hazel-local-copy.tar.gz
 cd hazel
-git checkout a0f7f67df7423fc84f39198ff46abacd84261e78
-git apply --whitespace=nowarn ../hazel.patch
-git add .; git commit -m "Hazel patch for Affect"
+git checkout 0936b5dc00b5d0b5802e7ca8e3dbd5afeafd970e
+git am --whitespace=nowarn ../hazel-patches/0001-Bumps-Iris-version-to-dev.2024-10-07.0.6dece417.patch
+git am --whitespace=nowarn ../hazel-patches/0001-Adds-a-Replace-e1-e2-construct.patch
+git am --whitespace=nowarn ../hazel-patches/0001-Add-IsContOS-unary-operation-and-specialised-shallow.patch
 opam install . 
 cd ..
 ```
